refactor: Replace Ground for CompleteMinimal

src/Examples/Tutorial/Refinement.v
@@ -20,27 +20,27 @@ Arguments refinement : simpl never.
 Tactic Notation "unfold_refinement" := unfold refinement; cbn.
 Tactic Notation "unfold_refinement" "in" hyp(H) := unfold refinement in H; cbn in H.
 
-#[export]
+#[export] 
 Instance refinableTransitive {A} `{Refinable A} : Transitive refinement := { transitivity := is_transitive }.
-#[export]
+#[export] 
 Instance refinableReflexive {A} `{Refinable A} : Reflexive refinement := { reflexivity := is_reflexive }.
 
-#[export]
+#[export] 
 Program Instance refinableFun {A B} `{Refinable A} `{Refinable B} : Refinable (A -> B) :=
   {
     refinement f g := forall a, f a ⊑ g a ;
   }.
-Next Obligation.
-  red; intros; etransitivity; eauto.
+Next Obligation. 
+  red; intros; etransitivity; eauto. 
 Qed.
 Next Obligation.
-  red; intros; reflexivity.
+  red; intros; reflexivity. 
 Qed.
 
 (***********************************)
 (*          Monotonous             *)
 (***********************************)
-Definition is_monotone {A B} `{Refinable A} `{Refinable B} (f : A -> B) :=
+Definition is_monotone {A B} `{Refinable A} `{Refinable B} (f : A -> B) := 
     forall a1 a2, a1 ⊑ a2 -> f a1 ⊑ f a2.
 
 Lemma fun_is_monotone : forall {A B} `{Refinable A} `{Refinable B},
@@ -52,7 +52,7 @@ Qed.
 Existing Class is_monotone.
 
 #[export] Hint Resolve fun_is_monotone : typeclass_instances.
-
+    
 (***********************************)
 (*          Complete               *)
 (***********************************)
@@ -70,7 +70,7 @@ Tactic Notation "unfold_complete" := unfold is_complete; cbn.
 #[export] Hint Extern 0 (@is_complete ?B _) => unfold B :  typeclass_instances.
 #[export] Hint Extern 0 (is_complete _) => unfold_complete : typeclass_instances.
 
-#[export]
+#[export] 
 Instance completeFun {A B} `{Complete A} `{Complete B} : Complete (A -> B) :=
   {
     is_complete f := forall a, is_complete a -> is_complete (f a) ;
@@ -85,18 +85,18 @@ Qed.
 
 #[export] Hint Resolve apply_complete : typeclass_instances.
 
-Lemma is_complete_const_fun : forall {A B} `{Complete A} `{Complete B} (b : B),
+Lemma is_complete_const_fun : forall {A B} `{Complete A} `{Complete B} (b : B), 
   is_complete b -> is_complete (fun _ : A => b).
-Proof.
+Proof. 
   intros ? ? ? ? ? ? b Hb. red; cbn. intros; eauto.
 Qed.
 
 #[export] Hint Resolve is_complete_const_fun : typeclass_instances.
 
 (***********************************)
-(*          Ground                 *)
+(*          CompleteMinimal        *)
 (***********************************)
-Class Ground (A : Type) `{Refinable A} `{Complete A} :=
+Class CompleteMinimal (A : Type) `{Refinable A} `{Complete A} :=
   {
     is_complete_minimal : forall a, is_complete a -> forall a', a' ⊑ a -> a' = a
   }.
@@ -114,8 +114,8 @@ Instance eqRefinable (A : Type) : Refinable A | 100 :=
   is_reflexive := ltac:(red; intros; reflexivity) ;
  |}.
 
-
-(* Makes complete instances where the complete predicate is always true.
+  
+(* Makes complete instances where the complete predicate is always true. 
   The premise is just to reuse the definition for other types with eq refinement.
 *)
 #[export]
@@ -131,10 +131,10 @@ exact I
 
 
 #[export]
-Instance eqGroundTrue (A : Type) (refEqA := eqRefinable A) (compA := eqCompleteTrue A) : Ground A | 100.
+Instance eqCompleteMinimalTrue (A : Type) (refEqA := eqRefinable A) (compA := eqCompleteTrue A) : CompleteMinimal A | 100.
 Proof. econstructor. eauto. Qed.
 
-
+  
 
 Section IncReformulation.
   Context {A} {HA: Refinable A} {HAC : Complete A}.
@@ -151,8 +151,8 @@ Section IncReformulation.
       recoverability_anti : forall (a : A), is_complete a -> P a -> ir_anti a
       }.
 
-  Arguments ir_mono P {IncRef} a.
-  Arguments ir_anti P {IncRef} a.
+  Arguments ir_mono P {IncRef} a. 
+  Arguments ir_anti P {IncRef} a. 
 
   Lemma complete_monotone_is_equivalent {P} `{IncRef P} : forall (a : A), is_complete a -> ir_mono P a <-> P a.
   Proof.
@@ -166,27 +166,27 @@ Section IncReformulation.
 
   Obligation Tactic :=  try now eauto.
 
-  #[export]
+  #[export] 
   Program Instance IncRefConst (P : Prop) : IncRef (fun a => P) := {
       ir_mono := fun _ => P ;
       ir_anti := fun _ => P ;
     }.
-
+  
   Obligation Tactic :=  try now intuition.
 
-  #[export]
-  Program Instance IncRefEq {B} `{HB : Ground B}
+  #[export] 
+  Program Instance IncRefEq {B} `{HB : CompleteMinimal B}
     (f g : A -> B) (Hcf : is_monotone f) (Hcg : is_monotone g)
     (Hcf' : is_complete f) (Hcg' : is_complete g)
     : IncRef (fun a => f a = g a) | 2
     := {
       ir_mono := fun a => exists b, b ⊑ f a /\ b ⊑ g a ;
-      ir_anti := fun a => is_complete (f a) /\ f a = g a ;
+      ir_anti := fun a => is_complete (f a) /\ f a = g a ; 
     }.
   Next Obligation.
     intros ? ? ? ? f g ? ? ? ? a1 a2 Hprec [b [? ?]].
     exists b. split.
-    - transitivity (f a1) ; auto.
+    - transitivity (f a1) ; auto. 
     - transitivity (g a1) ; auto.
   Qed.
   Next Obligation.
@@ -197,8 +197,8 @@ Section IncReformulation.
   Qed.
   Next Obligation.
   intros ? ? ? ? ? ? ? ? ? ? ? Hca.
-  cbn in *. eexists. split; try reflexivity. rewrite Hca; reflexivity.
-  Qed.
+  cbn in *. eexists. split; try reflexivity. rewrite Hca; reflexivity.  
+  Qed. 
   Next Obligation.
     intros ? ? ? ? ? ? ? ? ? ? ? ?.
     intros [b [Hb1 Hb2]].
@@ -207,9 +207,9 @@ Section IncReformulation.
     assumption.
   Qed.
 
-  #[export]
-  Program Instance IncRefEqL {B} `{HB : Ground B}
-    (f : A -> B) (Hcf : is_complete f) (Hmonof : is_monotone f)
+  #[export] 
+  Program Instance IncRefEqL {B} `{HB : CompleteMinimal B}
+    (f : A -> B) (Hcf : is_complete f) (Hmonof : is_monotone f) 
     (b : B) : IncRef (fun a => f a = b) | 1 := {
       ir_mono := fun a => b ⊑ f a ;
       ir_anti := fun a => is_complete (f a) /\ f a = b ;
@@ -219,7 +219,7 @@ Section IncReformulation.
     transitivity (f a1); try apply Hcf; eauto.
   Qed.
   Next Obligation.
-    intros ? ? ? ? ? ? Hmono b a1 a2 Hprec [? ?].
+    intros ? ? ? ? ? ? Hmono b a1 a2 Hprec [? ?]. 
     eapply is_complete_minimal in Hmono; eauto.
     rewrite Hmono; eauto.
   Qed.
@@ -231,8 +231,8 @@ Section IncReformulation.
     cbn. symmetry. eapply is_complete_minimal; eauto.
   Qed.
 
-  #[export]
-  Program Instance IncRefForall {B} {P : B -> A -> Prop} `{HPB : forall b, IncRef (P b)} :
+  #[export] 
+  Program Instance IncRefForall {B} {P : B -> A -> Prop} `{HPB : forall b, IncRef (P b)} :      
     IncRef (fun a => forall b, P b a) :=
     {
       ir_mono := fun a => forall b, ir_mono (P b) a ;
@@ -263,9 +263,9 @@ Section IncReformulation.
     intros B P HPB a Hac; simpl; intros HP b; eapply complete_antitone_is_equivalent...
   Qed.
 
-  #[export]
-  Program Instance IncRefExists {B} `{HB: Refinable B}
-    {P : B -> A -> Prop} `{HPB : forall b, IncRef (P b)}
+  #[export] 
+  Program Instance IncRefExists {B} `{HB: Refinable B} 
+    {P : B -> A -> Prop} `{HPB : forall b, IncRef (P b)} 
     : IncRef (fun a => exists b, P b a) :=
     {
       ir_mono := fun a => exists b, ir_mono (P b) a ;
@@ -296,8 +296,8 @@ Section IncReformulation.
       eapply complete_antitone_is_equivalent...
   Qed.
 
-  #[export]
-  Program Instance IncRefConj (P Q : A -> Prop) {HP : IncRef P} {HQ : IncRef Q} :
+  #[export] 
+  Program Instance IncRefConj (P Q : A -> Prop) {HP : IncRef P} {HQ : IncRef Q} :  
     IncRef (fun a => P a /\ Q a) :=
     {
       ir_mono := fun a => (ir_mono P a) /\ (ir_mono Q a) ;
@@ -326,8 +326,8 @@ Section IncReformulation.
     intros P Q HP HQ a Hac; simpl; intros [HP1 HQ1]; split; try eapply complete_antitone_is_equivalent...
   Qed.
 
-  #[export]
-  Program Instance IncRefDisj (P Q : A -> Prop) {HP : IncRef P} {HQ : IncRef Q} :
+  #[export] 
+  Program Instance IncRefDisj (P Q : A -> Prop) {HP : IncRef P} {HQ : IncRef Q} : 
     IncRef (fun a => P a \/ Q a) :=
     {
       ir_mono := fun a => (ir_mono P a) \/ (ir_mono Q a) ;
@@ -364,8 +364,8 @@ Section IncReformulation.
       try (now right; apply complete_antitone_is_equivalent; eauto).
   Qed.
 
-  #[export]
-  Program Instance IncRefArrow {P Q : A -> Prop} {HP : IncRef P} {HQ : IncRef Q} :
+  #[export] 
+  Program Instance IncRefArrow {P Q : A -> Prop} {HP : IncRef P} {HQ : IncRef Q} : 
     IncRef (fun a => P a -> Q a) :=
     {
       ir_mono := fun a => ir_anti P a -> ir_mono Q a ;
@@ -404,12 +404,12 @@ Section IncReformulation.
 
 End IncReformulation.
 
-Arguments ir_mono {A HA HAC} P {IncRef} _.
-Arguments ir_anti {A HA HAC} P {IncRef} _.
+Arguments ir_mono {A HA HAC} P {IncRef} _. 
+Arguments ir_anti {A HA HAC} P {IncRef} _. 
 
-Lemma IncRefEquiv : forall A `{Refinable A} `{Complete A} (P Q : A -> Prop) ,
-  IncRef P ->
-  (forall a, P a <-> Q a) ->
+Lemma IncRefEquiv : forall A `{Refinable A} `{Complete A} (P Q : A -> Prop) , 
+  IncRef P -> 
+  (forall a, P a <-> Q a) -> 
   IncRef Q.
 Proof.
   intros A HAR HAC P Q HPmono Hequiv.
@@ -418,24 +418,24 @@ Proof.
   - exact (ir_anti P).
   - eapply HPmono.(is_monotone_mono).
   - eapply HPmono.(is_antitone_anti).
-  - intros a Ha. now eapply approx_mono, Hequiv.
-  - intros a Ha. now eapply Hequiv, approx_anti.
+  - intros a Ha. now eapply approx_mono, Hequiv. 
+  - intros a Ha. now eapply Hequiv, approx_anti. 
   - intros a Hac.
     * intros HPa. apply Hequiv. eapply (complete_monotone_is_equivalent); eauto.
   - intros a Hac.
     * intros HQa. apply Hequiv in HQa. eapply (complete_antitone_is_equivalent); eauto.
 Qed.
 
-#[export]
-Instance IncRefEq_fun {A} `{Refinable A} `{Complete A}
-  {B} `{Refinable B}
+#[export] 
+Instance IncRefEq_fun {A} `{Refinable A} `{Complete A} 
+  {B} `{Refinable B} 
   {C} `{Refinable C}
-  (f g : A -> B -> C) {Hmono : IncRef (fun a => forall b, f a b = g a b)}
+  (f g : A -> B -> C) {Hmono : IncRef (fun a => forall b, f a b = g a b)} 
   : IncRef (fun a => f a = g a).
 Proof.
   eapply IncRefEquiv.
   - apply Hmono.
   - intros; split.
     * intros. apply functional_extensionality; eauto.
-    * intros ->; eauto.
+    * intros ->; eauto. 
 Defined.
